Change frames to include temporaries
Slightly restructure code to share local maps (maps of
variables/temporaries to values) between typing and semantics, so it can
be used in both typing contexts and frames.

Also makes VarMapsTo, addVar, etc shared between the two, for easier
future code.

src/Typing.v
@@ -1,51 +1,28 @@
-From Pony Require Import Language.
+From Pony Require Import Language LocalMap.
 
 Require Import Coq.FSets.FMapInterface.
 Require Import Coq.Structures.Equalities.
 
 Module Context (Map : WSfun).
 
-Module VarTempMap := Map DecidableVarTemp.
-Definition varTempMap := VarTempMap.t.
-
 Include Syntax.
 
-Definition context : Type := (varTempMap aliasedType).
+Module LocalMap := LocalMap Map.
+Include LocalMap.
 
-Definition contextKey : Type := VarTempMap.key.
+Definition context : Type := (LocalMap.t aliasedType).
 
 Definition sendableCtxt (gamma : context) : context :=
-  VarTempMap.fold
+  LocalMap.fold
     (fun var varType sendableMap =>
       match varType with
       | aType _ b =>
           if isSendable b
-            then VarTempMap.add var varType sendableMap
+            then LocalMap.add var varType sendableMap
             else sendableMap
       end)
-    (VarTempMap.empty aliasedType)
+    (LocalMap.empty aliasedType)
     gamma.
-
-Definition VarMapsTo (var : var) (aT : aliasedType) (gamma : context) : Prop :=
-  VarTempMap.MapsTo (inl var) aT gamma.
-
-Definition TempMapsTo (temp : temp) (aT : aliasedType) (gamma : context) : Prop :=
-  VarTempMap.MapsTo (inr temp) aT gamma.
-
-Definition VarIn (var : var) (gamma : context) : Prop :=
-  VarTempMap.In (inl var) gamma.
-
-Definition addVar (var : var) (aT : aliasedType) (gamma : context) : context :=
-  VarTempMap.add (inl var) aT gamma.
-
-Definition removeVar (var : var) (gamma : context) : context :=
-  VarTempMap.remove (inl var) gamma.
-
-Fixpoint removeMany (keys : list contextKey) (gamma : context) :=
-  match keys with
-  | h :: t => VarTempMap.remove h (removeMany t gamma)
-  | nil => gamma
-  end.
 
 End Context.
 
@@ -362,7 +339,7 @@ Inductive well_formed_expr { P : Program.program } : context -> expressionSeq ->
 
 (* For some method arguments, produce the corresponding typing context *)
 Definition argsToContext (args : arrayVarMap aliasedType) : context :=
-  ArrayVarMap.fold aliasedType (varTempMap aliasedType)
+  ArrayVarMap.fold aliasedType (LocalMap.t aliasedType)
     (fun key val ctxt => VarTempMap.add (inl key) val ctxt)
     args
     (VarTempMap.empty aliasedType).
