src/LocalMap.v
@@ -1,0 +1,26 @@
+From Pony Require Import Language.
+
+Require Import Coq.FSets.FMapInterface.
+
+Module LocalMap (Map : WSfun).
+
+Module VarTempMap := Map DecidableVarTemp.
+
+Include VarTempMap.
+
+Definition VarMapsTo { E : Type } (var : Syntax.var) (e : E) (m : t E) : Prop :=
+  VarTempMap.MapsTo (inl var) e m.
+
+Definition TempMapsTo { E : Type } (temp : Syntax.temp) (e : E) (m : t E) : Prop :=
+  VarTempMap.MapsTo (inr temp) e m.
+
+Definition VarIn { E : Type } (var : Syntax.var) (m : t E) : Prop :=
+  VarTempMap.In (inl var) m.
+
+Definition addVar { E : Type } (var : Syntax.var) (e : E) (m : t E) : t E :=
+  VarTempMap.add (inl var) e m.
+
+Definition removeVar { E : Type } (var : Syntax.var) (m : t E) : t E :=
+  VarTempMap.remove (inl var) m.
+
+End LocalMap.
